Logic/Modal/Standard/Kripke/GL/GL.lean
@@ -1,4 +1,3 @@
 import Logic.Modal.Standard.Kripke.GL.Completeness
 import Logic.Modal.Standard.Kripke.GL.Tree
 import Logic.Modal.Standard.Kripke.GL.MDP
-import Logic.Modal.Standard.Kripke.GL.Boxdot
