Logic/Modal/Standard/Kripke/Kripke.lean
@@ -10,5 +10,3 @@ import Logic.Modal.Standard.Kripke.Dot3
 import Logic.Modal.Standard.Kripke.S5
 import Logic.Modal.Standard.Kripke.GL.GL
 import Logic.Modal.Standard.Kripke.Grz.Grz
-
-import Logic.Modal.Standard.Kripke.ModalCompanion
