Logic/Modal/Standard/ModalCompanion/ModalCompanion.lean
@@ -1,0 +1,2 @@
+import Logic.Modal.Standard.ModalCompanion.Basic
+import Logic.Modal.Standard.ModalCompanion.GMT
